Make kraft_ineqScript.sml prettier

examples/computability/kolmog/kraft_ineqScript.sml
@@ -25,588 +25,692 @@ val _ = intLib.deprecate_int()
 
 
 
-val len_fun_def = Define`len_fun (A:bool list set) n = let strs = {s | (LENGTH s = n) /\ s IN A} in EXTREAL_SUM_IMAGE (\s. Normal (2 rpow (- &(LENGTH s)))) strs`
+Definition len_fun_def:
+  len_fun (A:bool list set) n =
+  let strs = {s | (LENGTH s = n) /\ s IN A}
+  in
+    EXTREAL_SUM_IMAGE (\s. Normal (2 rpow (- &(LENGTH s)))) strs
+End
 
 Theorem extreal_sum_image_finite_corr:
-  !P. FINITE P ==> !f x. (!y. (y IN P) ==> (f y = x)) ==> (SIGMA f P = &CARD P * x)
+  !P. FINITE P ==>
+      !f x. (!y. (y IN P) ==> (f y = x)) ==> (SIGMA f P = &CARD P * x)
 Proof
-  rw[] >> Cases_on`P = {}` >> simp[] 
+  rw[] >> Cases_on‘P = {}’ >> simp[]
   >- rw[extrealTheory.EXTREAL_SUM_IMAGE_THM, extrealTheory.mul_lzero] >>
-  `∃m. m∈P` by metis_tac[MEMBER_NOT_EMPTY] >> `x = f m` by fs[] >> rw[] >>
+  ‘∃m. m ∈ P’ by metis_tac[MEMBER_NOT_EMPTY] >> ‘x = f m’ by fs[] >> rw[] >>
   irule extrealTheory.EXTREAL_SUM_IMAGE_FINITE_SAME >> rw[] >>
   CCONTR_TAC >> fs[] >> fs[]
 QED
 
+Theorem bool_list_card[simp]:
+  CARD {s | LENGTH (s:bool list) = n} = 2**n
+Proof
+  Induct_on‘n’>>simp[LENGTH_CONS] >> qmatch_abbrev_tac‘CARD s = 2**(SUC n)’>>
+  ‘s = IMAGE (CONS T) {s | LENGTH s = n} ∪ IMAGE (CONS F) {s | LENGTH s = n}’
+    by (simp[Abbr‘s’,EXTENSION,EQ_IMP_THM] >> rw[] ) >>
+  simp[CARD_UNION_EQN,CARD_INJ_IMAGE,EXP] >>
+  qmatch_abbrev_tac‘(x:num)-y=x’ >>
+  ‘y=0’ suffices_by simp[] >> simp[Abbr‘y’,EXTENSION] >>Cases>>simp[]>>
+  metis_tac[]
+QED
 
-
-val bool_list_card = Q.store_thm("bool_list_card[simp]",
-`CARD {s | LENGTH (s:bool list) = n} = 2**n`,
-Induct_on`n`>>simp[LENGTH_CONS] >> qmatch_abbrev_tac`CARD s = 2**(SUC n)`>>
-`s = IMAGE (CONS T) {s | LENGTH s = n} UNION IMAGE (CONS F) {s | LENGTH s = n}` by
-  (simp[Abbr`s`,EXTENSION,EQ_IMP_THM] >> rw[] ) >> simp[CARD_UNION_EQN,CARD_INJ_IMAGE,EXP] >>
-qmatch_abbrev_tac`(x:num)-y=x` >> `y=0`suffices_by simp[] >> simp[Abbr`y`,EXTENSION] >>Cases>>simp[]>>
-metis_tac[]  )
-
-val len_fun_eq1 = Q.store_thm("len_fun_eq1",
-`SIGMA (\s. Normal (2 rpow -&LENGTH s)) {s | (LENGTH (s:bool list) = n)} = 1`,
-irule EQ_TRANS >>qexists_tac`&CARD {s | LENGTH (s:bool list) = n} * Normal(2 rpow (-&n))` >> conj_tac
+Theorem len_fun_eq1:
+  SIGMA (\s. Normal (2 rpow -&LENGTH s)) {s | (LENGTH (s:bool list) = n)} = 1
+Proof
+  irule EQ_TRANS >>
+  qexists_tac‘&CARD {s | LENGTH (s:bool list) = n} * Normal(2 rpow (-&n))’ >>
+  conj_tac
   >- (irule extreal_sum_image_finite_corr >> rw[])
-  >- (simp[extreal_of_num_def,extreal_mul_def,GSYM realTheory.REAL_OF_NUM_POW,GEN_RPOW,
-           GSYM RPOW_ADD,RPOW_0 ] ))
+  >- (simp[extreal_of_num_def,extreal_mul_def,GSYM realTheory.REAL_OF_NUM_POW,
+           GEN_RPOW, GSYM RPOW_ADD,RPOW_0 ] )
+QED
 
-val len_fun_le1 = Q.store_thm("len_fun_le1",
-`len_fun A n <= 1`,
-rw[len_fun_def] >> `{s | LENGTH s = n /\ s IN A} SUBSET {s|LENGTH s = n}` by simp[SUBSET_DEF] >>
-`FINITE {s | LENGTH s = n /\ s IN A}` by metis_tac[SUBSET_FINITE_I,finite_bool_list_n] >>
-ASSUME_TAC len_fun_eq1 >> pop_assum(SUBST1_TAC o SYM)>> irule EXTREAL_SUM_IMAGE_MONO_SET >>
-simp[finite_bool_list_n] >> rw[extreal_of_num_def,extreal_le_def] >>
-`0r < 2 `suffices_by(strip_tac >> drule RPOW_POS_LT >> simp[realTheory.REAL_LE_LT]) >>
-simp[] )
+Theorem len_fun_le1:
+  len_fun A n <= 1
+Proof
+  rw[len_fun_def] >>
+  ‘{s | LENGTH s = n /\ s IN A} SUBSET {s|LENGTH s = n}’ by simp[SUBSET_DEF] >>
+  ‘FINITE {s | LENGTH s = n /\ s IN A}’
+    by metis_tac[SUBSET_FINITE_I,finite_bool_list_n] >>
+  ASSUME_TAC len_fun_eq1 >> pop_assum(SUBST1_TAC o SYM)>>
+  irule EXTREAL_SUM_IMAGE_MONO_SET >>
+  simp[finite_bool_list_n] >> rw[extreal_of_num_def,extreal_le_def] >>
+  ‘0r < 2 ’suffices_by(strip_tac >> drule RPOW_POS_LT >>
+                       simp[realTheory.REAL_LE_LT]) >>
+  simp[]
+QED
 
 (* Traditional bool list to num *)
-val rev_fpow = Q.store_thm("rev_fpow[simp]",
-`REVERSE (Fpow n) = Fpow n`,
-simp[Fpow_def,listTheory.REVERSE_GENLIST,combinTheory.K_DEF])
+Theorem rev_fpow[simp]: REVERSE (Fpow n) = Fpow n
+Proof simp[Fpow_def,listTheory.REVERSE_GENLIST,combinTheory.K_DEF]
+QED
 
-val rev_tpow = Q.store_thm("rev_tpow[simp]",
-`REVERSE (Tpow n) = Tpow n`,
-simp[Tpow_def,listTheory.REVERSE_GENLIST,combinTheory.K_DEF])
+Theorem rev_tpow[simp]: REVERSE (Tpow n) = Tpow n
+Proof simp[Tpow_def,listTheory.REVERSE_GENLIST,combinTheory.K_DEF]
+QED
 
+Definition tbl2n_def[simp]:
+  tbl2n [] = 0n /\
+  tbl2n (T::t) = 2*tbl2n t + 1 /\
+  tbl2n (F::t) = 2*tbl2n t
+End
 
-val tbl2n_def = Define`tbl2n [] = 0n /\ tbl2n (T::t) = 2*tbl2n t + 1 /\ tbl2n (F::t) = 2*tbl2n t`
+Overload TBL2N = “\l. tbl2n (REVERSE l)”
 
-val _ = export_rewrites["tbl2n_def"]
+Definition inv_tbl2n_def:
+  inv_tbl2n 0n = [] /\
+  inv_tbl2n a = if EVEN a then [F]++(inv_tbl2n (a DIV 2))
+                else [T]++(inv_tbl2n ((a-1) DIV 2 ))
+Termination
+  WF_REL_TAC‘$<’ >> rw[]>>
+  irule LESS_EQ_LESS_TRANS >> qexists_tac‘v’ >> ‘0<2n’ by simp[] >>
+  rw[DIV_LE_MONOTONE,DIV_LESS,DIV_LESS_EQ]
+End
 
-val _ = overload_on("TBL2N",``\l. tbl2n (REVERSE l)``)
+Theorem tbl2n_inv_tbl2n[simp]:
+  tbl2n (inv_tbl2n n) = n
+Proof
+  completeInduct_on ‘n’ >> Cases_on‘n’ >> simp[tbl2n_def,inv_tbl2n_def] >>
+  Cases_on‘EVEN (SUC n')’ >>
+  simp[tbl2n_def]
+  >- (‘2 * (SUC n' DIV 2) = (SUC n' DIV 2)*2’ by simp[MULT_COMM] >>
+      ‘0<2n’ by simp[] >>
+      ‘SUC n' MOD 2=0’ by metis_tac[EVEN_MOD2] >>
+      ‘SUC n' DIV 2 * 2 + SUC n' MOD 2 = SUC n'’ by metis_tac[GSYM DIVISION] >>
+      fs[])
+  >- (‘0<2n’ by simp[] >> ‘n' DIV 2 <= n'’ by simp[DIV_LESS_EQ] >>
+      ‘n' DIV 2 < SUC n'’ by
+        simp[LESS_EQ_IMP_LESS_SUC] >> fs[] >>
+      ‘EVEN n'’ by metis_tac[ODD,EVEN_OR_ODD] >>
+      ‘2 * (n' DIV 2) =  (n' DIV 2)*2’ by simp[MULT_COMM] >> ‘0<2n’ by simp[] >>
+      ‘n' MOD 2=0’ by metis_tac[EVEN_MOD2] >>
+      ‘n' DIV 2 * 2 + n' MOD 2 = n'’ by metis_tac[GSYM DIVISION] >> fs[] )
+QED
 
-val inv_tbl2n_def = tDefine"inv_tbl2n"`inv_tbl2n 0n = [] /\
-                           inv_tbl2n a = if EVEN a
-                                         then [F]++(inv_tbl2n (a DIV 2))
-                                         else [T]++(inv_tbl2n ((a-1) DIV 2 ))`
-(WF_REL_TAC`$<` >> rw[]>>
-irule LESS_EQ_LESS_TRANS >> qexists_tac`v` >> `0<2n` by simp[] >> rw[DIV_LE_MONOTONE,DIV_LESS,DIV_LESS_EQ])
+Definition interval_bl_def:
+  interval_bl l = (&(TBL2N l) *(2 rpow -&LENGTH l),(2 rpow -&LENGTH l))
+End
 
-val tbl2n_inv_tbl2n = Q.store_thm("tbl2n_inv_tbl2n",
-`tbl2n (inv_tbl2n n) = n`,
-completeInduct_on `n` >> Cases_on`n` >> simp[tbl2n_def,inv_tbl2n_def] >> Cases_on`EVEN (SUC n')` >>
-simp[tbl2n_def]
-  >- (`2 * (SUC n' DIV 2) =  (SUC n' DIV 2)*2` by simp[MULT_COMM] >> `0<2n` by simp[] >>
-       `SUC n' MOD 2=0` by metis_tac[EVEN_MOD2] >>
-       `SUC n' DIV 2 * 2 + SUC n' MOD 2 = SUC n'` by metis_tac[GSYM DIVISION] >> fs[])
-  >- (`0<2n` by simp[] >> `n' DIV 2 <= n'` by simp[DIV_LESS_EQ] >> `n' DIV 2 < SUC n'` by
-        simp[LESS_EQ_IMP_LESS_SUC] >> fs[] >> `EVEN n'` by metis_tac[ODD,EVEN_OR_ODD] >>
-       `2 * (n' DIV 2) =  (n' DIV 2)*2` by simp[MULT_COMM] >> `0<2n` by simp[] >>
-       `n' MOD 2=0` by metis_tac[EVEN_MOD2] >>
-       `n' DIV 2 * 2 + n' MOD 2 = n'` by metis_tac[GSYM DIVISION] >> fs[] ) )
+Definition disjoint_interval_def:
+  disjoint_interval ((m:real),i) (n,j) <=>
+  DISJOINT {r|m<=r /\ r<m+i} {r|n<=r /\ r<n+j}
+End
 
-val interval_bl_def = Define`interval_bl l = (&(TBL2N l) *(2 rpow -&LENGTH l),(2 rpow -&LENGTH l))`
+Theorem tbl2n_exp2: tbl2n i * 2 ** n = tbl2n ((Fpow n)++i)
+Proof
+  rw[Fpow_def] >> Induct_on‘n’ >> simp[tbl2n_def,EXP,GENLIST_CONS]
+QED
 
-val disjoint_interval_def = Define`disjoint_interval ((m:real),i) (n,j) <=>
-                                   DISJOINT {r|m<=r /\ r<m+i} {r|n<=r /\ r<n+j}`
+Theorem TBL2N_exp2: TBL2N i * 2 ** n = TBL2N (i++(Fpow n))
+Proof
+  simp[REVERSE_APPEND] >> rw[Fpow_def] >> Induct_on‘n’ >>
+  simp[tbl2n_def,EXP,GENLIST_CONS]
+QED
 
-val tbl2n_exp2 = Q.store_thm("tbl2n_exp2",
-`tbl2n i * 2 ** n = tbl2n ((Fpow n)++i)`,
-rw[Fpow_def] >> Induct_on`n` >> simp[tbl2n_def,EXP,GENLIST_CONS])
+Theorem tbl2n_lead0s[simp]: tbl2n (x ++ Fpow n) = tbl2n x
+Proof
+  Induct_on‘x’ >> simp[tbl2n_def]
+  >- (‘tbl2n (Fpow n ++ []) = tbl2n (Fpow n )’ by simp[] >>
+      ‘tbl2n (Fpow n ++ []) = (tbl2n []) *2**n’ by metis_tac[GSYM tbl2n_exp2] >>
+      fs[tbl2n_def])
+  >- (Cases_on ‘h’ >> simp[tbl2n_def])
+QED
 
-val TBL2N_exp2 = Q.store_thm("TBL2N_exp2",
-`TBL2N i * 2 ** n = TBL2N (i++(Fpow n))`,
-simp[REVERSE_APPEND] >> rw[Fpow_def] >> Induct_on`n` >> simp[tbl2n_def,EXP,GENLIST_CONS])
+Theorem tbl2n_fpow[simp]: tbl2n (Fpow n) = 0
+Proof simp[Fpow_def] >> Induct_on‘n’ >> simp[GENLIST_CONS]
+QED
 
+Theorem len_fpow[simp]: LENGTH (Fpow n) = n
+Proof simp[Fpow_def]
+QED
 
-val tbl2n_lead0s = Q.store_thm("tbl2n_lead0s[simp]",
-`tbl2n (x ++ Fpow n) = tbl2n x`,
-Induct_on`x` >> simp[tbl2n_def]
-  >- (`tbl2n (Fpow n ++ []) = tbl2n (Fpow n )` by simp[] >>
-      `tbl2n (Fpow n ++ []) = (tbl2n []) *2**n` by metis_tac[GSYM tbl2n_exp2] >> fs[tbl2n_def])
-  >- (Cases_on `h` >> simp[tbl2n_def])  )
+Theorem TBL2N_lead0s[simp]: TBL2N (Fpow n ++ x) = TBL2N x
+Proof simp[REVERSE_APPEND]
+QED
 
-val tbl2n_fpow = Q.store_thm("tbl2n_fpow[simp]",
-`tbl2n (Fpow n) = 0`,
-simp[Fpow_def] >> Induct_on`n` >> simp[GENLIST_CONS])
+Theorem tbl2n_append_1:
+  tbl2n (x++[e]) = if e then 2**(LENGTH x) + (tbl2n x) else tbl2n x
+Proof
+  Induct_on‘x’ >> simp[] >- (Cases_on‘e’ >> simp[]) >> Cases_on‘h’ >> simp[] >>
+  rw[] >> simp[EXP]
+QED
 
-val len_fpow = Q.store_thm("len_fpow[simp]",
-`LENGTH (Fpow n) = n`,
-simp[Fpow_def])
+Theorem tbl2n_append_full: !y. tbl2n (x++y) = tbl2n x + 2**(LENGTH x) * tbl2n y
+Proof
+  Induct_on‘x’ >> simp[] >> Cases_on‘h’ >> simp[EXP]
+QED
 
-val TBL2N_lead0s = Q.store_thm("TBL2N_lead0s[simp]",
-`TBL2N (Fpow n ++ x) = TBL2N x`,
-simp[REVERSE_APPEND]  )
+Theorem tbl2n_ub[simp]: tbl2n l < 2**(LENGTH l)
+Proof Induct_on‘l’ >> simp[] >> Cases_on‘h’ >> simp[EXP]
+QED
 
-val tbl2n_append_1 = Q.store_thm("tbl2n_append_1",
-`tbl2n (x++[e]) = if e then 2**(LENGTH x) + (tbl2n x) else tbl2n x`,
-Induct_on`x` >> simp[] >- (Cases_on`e` >> simp[]) >> Cases_on`h` >> simp[] >> rw[] >> simp[EXP] );
+Theorem TBL2N_ub[simp]: TBL2N l < 2**(LENGTH l)
+Proof metis_tac[tbl2n_ub,LENGTH_REVERSE]
+QED
 
-val tbl2n_append_full = Q.store_thm("tbl2n_append_full",
-`!y. tbl2n (x++y) = tbl2n x + 2**(LENGTH x) * tbl2n y`,
-Induct_on`x` >> simp[] >> Cases_on`h` >> simp[EXP])
+Theorem TBL2N_inj_len:
+  !x y.(LENGTH x = LENGTH y) ==> (TBL2N x = TBL2N y <=> x=y)
+Proof
+  Induct_on‘x’ >> simp[] >> Cases_on‘y’ >> simp[] >> rw[tbl2n_append_1] >>
+  ‘TBL2N t < 2** LENGTH t’ by  (metis_tac[tbl2n_ub,LENGTH_REVERSE]) >>
+  ‘TBL2N x < 2** LENGTH t’ by  (metis_tac[tbl2n_ub,LENGTH_REVERSE]) >>simp[]
+QED
 
-val tbl2n_ub = Q.store_thm("tbl2n_ub[simp]",
-`tbl2n l < 2**(LENGTH l)`,
-Induct_on`l` >> simp[] >> Cases_on`h` >> simp[EXP]);
+Theorem TBL2N_lem1:
+  !d. d<2**D ==>
+      ?l. TBL2N l = d /\ LENGTH l = D /\
+          TBL2N (i++Fpow D) +d = TBL2N (i++l)
+Proof
+  Induct_on‘D’ >- simp[Fpow_def] >> rw[EXP] >> Cases_on‘d<2**D’ >> fs[]
+  >- (res_tac >> qexists_tac‘F::l’ >> simp[] >> fs[REVERSE_APPEND] >>
+      simp[tbl2n_append_full])
+  >- (qabbrev_tac‘d0=d-2**D’ >> ‘d0 < 2**D’ by simp[Abbr‘d0’] >> res_tac >>
+      qexists_tac‘T::l’ >>
+      simp[] >>fs[REVERSE_APPEND] >> simp[tbl2n_append_full] >> simp[Abbr‘d0’] )
+QED
 
-val TBL2N_ub = Q.store_thm("TBL2N_ub[simp]",
-`TBL2N l < 2**(LENGTH l)`,
-metis_tac[tbl2n_ub,LENGTH_REVERSE]);
+Theorem disjoint_pf_lem1:
+  TBL2N i * 2 ** (LENGTH j - LENGTH i) <= TBL2N j /\
+  TBL2N j < (TBL2N i + 1) * 2 ** (LENGTH j - LENGTH i) /\
+  LENGTH i < LENGTH j ==>
+  i ≺ j
+Proof
+  rw[TBL2N_exp2] >> qabbrev_tac‘D=LENGTH j − LENGTH i’ >>
+  ‘TBL2N (i ++ Fpow D) + (TBL2N j-TBL2N (i ++ Fpow D)) = TBL2N j’ by simp[] >>
+  qabbrev_tac‘d=TBL2N j-TBL2N (i ++ Fpow D)’ >>
+  ‘d<2**D’
+    by (fs[RIGHT_ADD_DISTRIB] >>
+        ‘TBL2N j - TBL2N i * 2 ** D < 2 ** D’ by simp[] >>
+        ‘TBL2N j − TBL2N (i ++ Fpow D) < 2**D’ by simp[GSYM TBL2N_exp2] >>
+        fs[Abbr‘d’] ) >>
+  ‘?l. TBL2N l = d /\ LENGTH l = D /\ TBL2N (i++Fpow D) +d = TBL2N (i++l)’
+    by simp[TBL2N_lem1] >>
+  ‘TBL2N (i ++ l) = TBL2N j’ by simp[] >>
+  ‘LENGTH (i++l) = LENGTH j’ by simp[Abbr‘D’] >>
+  ‘i++l = j’ by metis_tac[TBL2N_inj_len] >> ‘0<LENGTH l’ by simp[Abbr‘D’] >>
+  metis_tac[prefix_lem1]
+QED
 
+Theorem tbl2n_append:
+  tbl2n (p++s) = 2**LENGTH p * (tbl2n s) +tbl2n p
+Proof
+  Induct_on‘p’ >> simp[] >> Cases_on‘h’ >> rw[GSYM ADD1,EXP,LEFT_ADD_DISTRIB]
+QED
 
-val TBL2N_inj_len = Q.store_thm("TBL2N_inj_len",
-`!x y.(LENGTH x = LENGTH y) ==> (TBL2N x = TBL2N y <=> x=y)`,
-Induct_on`x` >> simp[] >> Cases_on`y` >> simp[] >> rw[tbl2n_append_1] >>
-`TBL2N t < 2** LENGTH t` by  (metis_tac[tbl2n_ub,LENGTH_REVERSE]) >>
-`TBL2N x < 2** LENGTH t` by  (metis_tac[tbl2n_ub,LENGTH_REVERSE]) >>simp[]);
+Theorem TBL2N_append:
+  TBL2N (p++s) = 2**LENGTH s * (TBL2N p) +TBL2N s
+Proof simp[REVERSE_APPEND,tbl2n_append]
+QED
 
-val TBL2N_lem1 = Q.store_thm("TBL2N_lem1",
-`!d. d<2**D ==> ?l. TBL2N l = d /\ LENGTH l = D /\ TBL2N (i++Fpow D) +d = TBL2N (i++l)`,
-Induct_on`D` >- simp[Fpow_def] >> rw[EXP] >> Cases_on`d<2**D` >> fs[]
-  >- (res_tac >> qexists_tac`F::l` >> simp[] >> fs[REVERSE_APPEND] >> simp[tbl2n_append_full])
-  >- (qabbrev_tac`d0=d-2**D` >> `d0 < 2**D` by simp[Abbr`d0`] >> res_tac >> qexists_tac`T::l` >>
-      simp[] >>fs[REVERSE_APPEND] >> simp[tbl2n_append_full] >> simp[Abbr`d0`] ) )
+Theorem disjoint_prefix_free:
+  prefix_free P <=>
+  let is = IMAGE interval_bl P
+  in
+    !i1 i2. i1 IN is /\ i2 IN is /\ i1<>i2 ==> disjoint_interval i1 i2
+Proof
+  rw[EQ_IMP_THM]
+  >- (rename[‘interval_bl i = interval_bl j’] >>
+      ‘~(i ≺ j) /\ ~(j ≺ i)/\ i<>j’ by metis_tac[prefix_free_def] >>
+      fs[interval_bl_def,disjoint_interval_def,DISJOINT_DEF,EXTENSION] >>
+      rw[GSYM DISJ_ASSOC] >> rw[DECIDE“~p\/q <=> p==>q”] >> strip_tac >>
+      ‘LENGTH i <> LENGTH j’
+        by (strip_tac >> fs[] >> qabbrev_tac‘M = 2 rpow -&LENGTH j’ >>
+            ‘&TBL2N i * M < &TBL2N j * M + M’ by metis_tac[REAL_LET_TRANS] >>
+            ‘&TBL2N j * M < &TBL2N i * M + M’ by metis_tac[REAL_LET_TRANS] >>
+            ‘&TBL2N i * M + M = (&TBL2N i + 1) * M’
+              by metis_tac[REAL_ADD_RDISTRIB,REAL_MUL_LID] >>
+            ‘&TBL2N j * M + M = (&TBL2N j + 1) * M’
+              by metis_tac[REAL_ADD_RDISTRIB,REAL_MUL_LID] >> fs[] >>
+            ‘(0:real)<2’ by fs[] >> ‘0<M’ by metis_tac[RPOW_POS_LT] >>
+            ‘((&TBL2N i) :real) < &(TBL2N j + 1)’ by fs[REAL_LT_RMUL] >>
+            ‘((&TBL2N j):real) < &(TBL2N i + 1)’ by fs[REAL_LT_RMUL] >> fs[]) >>
+      wlog_tac ‘LENGTH i < LENGTH j’ [‘i’,‘j’,‘x’]
+      >- (‘LENGTH j < LENGTH i’ by simp[] >> metis_tac[]) >>
+      ‘&TBL2N i * 2 rpow -&LENGTH i <
+       &TBL2N j * 2 rpow -&LENGTH j + 2 rpow -&LENGTH j’
+        by metis_tac[REAL_LET_TRANS]>>
+      ‘&TBL2N i * 2 rpow -&LENGTH i < (&TBL2N j +1) * 2 rpow -&LENGTH j’ by
+        metis_tac[REAL_ADD_RDISTRIB,REAL_MUL_LID] >> ‘(0:real)<2’ by fs[] >>
+      ‘&TBL2N i * 2 rpow  -&LENGTH i * 2 rpow &LENGTH j <
+       (&TBL2N j +1)  * 2 rpow -&LENGTH j  * 2 rpow &LENGTH j’ by
+        metis_tac[RPOW_POS_LT,REAL_LT_RMUL] >>
+      fs[GSYM REAL_MUL_ASSOC,GSYM RPOW_ADD,RPOW_0,add_ints] >> rfs[]>>
+      ‘&TBL2N j * 2 rpow -&LENGTH j <
+       &TBL2N i * 2 rpow -&LENGTH i + 2 rpow -&LENGTH i’ by
+        metis_tac[REAL_LET_TRANS] >>
+      ‘&TBL2N j * 2 rpow -&LENGTH j < (&TBL2N i +1) * 2 rpow -&LENGTH i’ by
+        metis_tac[REAL_ADD_RDISTRIB,REAL_MUL_LID] >> ‘(0:real)<2’ by fs[] >>
+      ‘&TBL2N j * 2 rpow  -&LENGTH j * 2 rpow &LENGTH j <
+       (&TBL2N i +1)  * 2 rpow -&LENGTH i  * 2 rpow &LENGTH j’ by
+        metis_tac[RPOW_POS_LT,REAL_LT_RMUL] >>
+      fs[GSYM REAL_MUL_ASSOC,GSYM RPOW_ADD,RPOW_0,add_ints] >> rfs[] >>
+      qabbrev_tac‘D=LENGTH j − LENGTH i’ >> qabbrev_tac‘ii= TBL2N i’ >>
+      qabbrev_tac‘jj= TBL2N j’ >> fs[GSYM GEN_RPOW,REAL_OF_NUM_POW] >>
+      fs[disjoint_pf_lem1])
+  >- (fs[prefix_free_def,PULL_EXISTS] >>rw[] >>
+      strip_tac >>
+      ‘interval_bl a <> interval_bl b’ by
+        (fs[interval_bl_def] >> rw[] >>
+         ‘LENGTH a < LENGTH b’ by simp[prefix_length_lt]>>
+         ‘real_of_num (LENGTH a) < real_of_num (LENGTH b)’ by fs[REAL_LT] >>
+         ‘-(real_of_num (LENGTH b)) < -(real_of_num(LENGTH a))’
+           by fs[REAL_LT_NEG] >>
+         ‘1<(2:real)’ by simp[]>>
+         ‘2 rpow -&LENGTH b < 2 rpow -&LENGTH a’ by fs[RPOW_LT]>>
+         fs[REAL_LT_IMP_NE])>>
+      first_x_assum drule_all >>
+      fs[interval_bl_def,disjoint_interval_def] >> rw[DISJOINT_DEF,EXTENSION] >>
+      qexists_tac‘&TBL2N b * 2 rpow -&LENGTH b’ >> rw[]
+      >- (‘0<2 rpow &LENGTH b’ by fs[RPOW_POS_LT] >>
+          drule_then (ONCE_REWRITE_TAC o list_of_singleton o GSYM)
+                     REAL_LE_RMUL >>
+          fs[GSYM REAL_MUL_ASSOC,GSYM RPOW_ADD,RPOW_0,add_ints]>>
+          drule_then assume_tac prefix_length_lt >> simp[] >>
+          fs[GSYM GEN_RPOW,REAL_OF_NUM_POW] >> fs[prefix_append,TBL2N_append]  )
+      >- (‘0<2 rpow &LENGTH b’ by fs[RPOW_POS_LT] >>
+          drule_then (ONCE_REWRITE_TAC o list_of_singleton o GSYM)
+                     REAL_LT_RMUL >>
+          drule_then assume_tac prefix_length_lt >>
+          fs[GSYM REAL_MUL_ASSOC,GSYM RPOW_ADD,RPOW_0,add_ints,
+             REAL_ADD_RDISTRIB,GSYM GEN_RPOW,REAL_OF_NUM_POW] >>
+          fs[prefix_append,TBL2N_append] )
+      >- (rw[REAL_LT_ADDR] >> ‘0<(2:real)’ by simp[] >> fs[RPOW_POS_LT]) )
+QED
 
+Theorem size_of_interval_bl:
+  Normal (SND (interval_bl y))  = Normal (2 rpow -&LENGTH y)
+Proof rw[interval_bl_def]
+QED
 
+Theorem TBL2N_append_sing_ub:
+  &(TBL2N (a++[h]) + 1)*2 rpow (-1) <= &(TBL2N a + 1)
+Proof
+  ‘&(2 * TBL2N a + 2) * 2 rpow -1 <= &(TBL2N a + 1)’
+    by (‘&(2 * TBL2N a + 2) * 2 rpow -1 = &(2*(TBL2N a + 1)) * 2 rpow -1’
+          by fs[GSYM LEFT_ADD_DISTRIB]>>
+        ‘_ = 2 * &(TBL2N a + 1) * 2 rpow -1’ by fs[REAL_MUL] >>
+        ‘_ = &(TBL2N a + 1)*(2 rpow 1 * 2 rpow -1)’
+          by fs[AC REAL_MUL_ASSOC REAL_MUL_COMM,RPOW_1]>>
+        ‘_ = &(TBL2N a + 1) * 2 rpow (1+ -1)’ by fs[RPOW_ADD] >>
+        fs[RPOW_0,REAL_ADD_RINV]  ) >>
+  Cases_on‘h’ >> rw[TBL2N_append] >>
+  ‘&(2 * TBL2N a + 1) * 2 rpow -1 <= &(2 * TBL2N a + 2) * 2 rpow -1’
+    by (irule REAL_LE_RMUL_IMP >> rw[RPOW_POS_LT,REAL_LE_LT]) >>
+  irule REAL_LE_TRANS >> qexists_tac‘&(2 * TBL2N a + 2) * 2 rpow -1’ >> rw[]
+QED
 
-val disjoint_pf_lem1 = Q.store_thm("disjoint_pf_lem1",
-`(TBL2N i * 2 ** (LENGTH j - LENGTH i) <= TBL2N j) /\ (TBL2N j < (TBL2N i + 1) * 2 ** (LENGTH j - LENGTH i)) /\ (LENGTH i < LENGTH j) ==> i ≺ j`,
-rw[TBL2N_exp2] >> qabbrev_tac`D=LENGTH j − LENGTH i` >>
-`TBL2N (i ++ Fpow D) + (TBL2N j-TBL2N (i ++ Fpow D)) = TBL2N j` by simp[] >>
-qabbrev_tac`d=TBL2N j-TBL2N (i ++ Fpow D)` >> `d<2**D` by (fs[RIGHT_ADD_DISTRIB] >>
-  `TBL2N j - TBL2N i * 2 ** D < 2 ** D` by simp[] >>
-  `TBL2N j − TBL2N (i ++ Fpow D) < 2**D` by simp[GSYM TBL2N_exp2] >> fs[Abbr`d`] ) >>
-`?l. TBL2N l = d /\ LENGTH l = D /\ TBL2N (i++Fpow D) +d = TBL2N (i++l)` by simp[TBL2N_lem1] >>
-`TBL2N (i ++ l) = TBL2N j` by simp[] >> `LENGTH (i++l) = LENGTH j` by simp[Abbr`D`] >>
-`i++l = j` by metis_tac[TBL2N_inj_len] >> `0<LENGTH l` by simp[Abbr`D`] >> metis_tac[prefix_lem1] )
+Theorem interval_bl_bounds:
+  0 ≤ FST (interval_bl a) /\ FST (interval_bl a) + SND (interval_bl a) ≤ 1
+Proof
+  rw[]
+  >- (fs[interval_bl_def] >> ‘(0:real)<= &TBL2N a’ by fs[tbl2n_def] >>
+      ‘(0:real)<2’ by simp[] >>
+      ‘0<2 rpow -&LENGTH a’ by fs[RPOW_POS_LT] >>
+      metis_tac[util_probTheory.REAL_LE_LT_MUL] )
+  >- (fs[interval_bl_def] >>
+      ‘&TBL2N a * 2 rpow -&LENGTH a + 2 rpow -&LENGTH a =
+       (&TBL2N a +1)* 2 rpow -&LENGTH a’
+        by fs[REAL_RDISTRIB] >> pop_assum SUBST1_TAC >>
+      ‘0<2 rpow &LENGTH a’ by fs[RPOW_POS_LT] >>
+      drule_then (ONCE_REWRITE_TAC o list_of_singleton o GSYM) REAL_LE_RMUL >>
+      simp[GSYM REAL_MUL_ASSOC,GSYM RPOW_ADD,RPOW_0,GSYM GEN_RPOW,
+           REAL_OF_NUM_POW] >>
+      (TBL2N_ub |> Q.INST [‘l’|->‘a’] |> assume_tac) >> simp[]  )
+QED
 
+Definition bls_size_def:
+  bls_size (P:bool list -> bool) n =
+  SIGMA (\s. (2 rpow -&LENGTH s)) {x|x IN P /\ LENGTH x < n }
+End
 
+Theorem finite_and:
+  FINITE {s| P s} ==> FINITE {s|  Q s /\ P s}
+Proof
+  rw[] >> ‘{s | Q s /\ P s} = {s | Q s}  INTER {s | P s}’ by fs[INTER_DEF] >>
+  fs[FINITE_INTER]
+QED
 
-
-val tbl2n_append = Q.store_thm("tbl2n_append",
-`tbl2n (p++s) = 2**LENGTH p * (tbl2n s) +tbl2n p`,
-Induct_on`p` >> simp[] >> Cases_on`h` >> rw[GSYM ADD1,EXP,LEFT_ADD_DISTRIB] )
-
-val TBL2N_append = Q.store_thm("TBL2N_append",
-`TBL2N (p++s) = 2**LENGTH s * (TBL2N p) +TBL2N s`,
-simp[REVERSE_APPEND,tbl2n_append])
-
-
-
-val disjoint_prefix_free = Q.store_thm("disjoint_prefix_free",
-`prefix_free P <=> let is = IMAGE interval_bl P in !i1 i2. i1 IN is /\ i2 IN is /\ i1<>i2 ==> disjoint_interval i1 i2`,
-rw[EQ_IMP_THM]
->- (rename[`interval_bl i = interval_bl j`] >>
-    `~(i ≺ j) /\ ~(j ≺ i)/\ i<>j` by metis_tac[prefix_free_def] >>
-    fs[interval_bl_def,disjoint_interval_def,DISJOINT_DEF,EXTENSION] >>
-    rw[GSYM DISJ_ASSOC] >> rw[DECIDE``~p\/q <=> p==>q``] >> strip_tac >>
-    `LENGTH i <> LENGTH j` by (strip_tac >> fs[] >> qabbrev_tac`M = 2 rpow -&LENGTH j` >>
-      `&TBL2N i * M < &TBL2N j * M + M` by metis_tac[REAL_LET_TRANS] >>
-      `&TBL2N j * M < &TBL2N i * M + M` by metis_tac[REAL_LET_TRANS] >>
-      `&TBL2N i * M + M = (&TBL2N i + 1) * M` by metis_tac[REAL_ADD_RDISTRIB,REAL_MUL_LID] >>
-      `&TBL2N j * M + M = (&TBL2N j + 1) * M` by metis_tac[REAL_ADD_RDISTRIB,REAL_MUL_LID] >> fs[] >>
-      `(0:real)<2` by fs[] >> `0<M` by metis_tac[RPOW_POS_LT] >>
-      `((&TBL2N i) :real) < &(TBL2N j + 1)` by fs[REAL_LT_RMUL] >>
-      `((&TBL2N j):real) < &(TBL2N i + 1)` by fs[REAL_LT_RMUL] >> fs[] ) >>
-    wlog_tac `LENGTH i < LENGTH j` [`i`,`j`,`x`] >- (`LENGTH j < LENGTH i` by simp[] >> metis_tac[])>>
-    `&TBL2N i * 2 rpow -&LENGTH i < &TBL2N j * 2 rpow -&LENGTH j + 2 rpow -&LENGTH j` by
-      metis_tac[REAL_LET_TRANS]>>
-    `&TBL2N i * 2 rpow -&LENGTH i < (&TBL2N j +1) * 2 rpow -&LENGTH j` by
-      metis_tac[REAL_ADD_RDISTRIB,REAL_MUL_LID] >> `(0:real)<2` by fs[] >>
-    `&TBL2N i * 2 rpow  -&LENGTH i * 2 rpow &LENGTH j <
-     (&TBL2N j +1)  * 2 rpow -&LENGTH j  * 2 rpow &LENGTH j` by
-       metis_tac[RPOW_POS_LT,REAL_LT_RMUL] >>
-    fs[GSYM REAL_MUL_ASSOC,GSYM RPOW_ADD,RPOW_0,add_ints] >> rfs[]>>
-    `&TBL2N j * 2 rpow -&LENGTH j < &TBL2N i * 2 rpow -&LENGTH i + 2 rpow -&LENGTH i` by
-      metis_tac[REAL_LET_TRANS] >>
-    `&TBL2N j * 2 rpow -&LENGTH j < (&TBL2N i +1) * 2 rpow -&LENGTH i` by
-      metis_tac[REAL_ADD_RDISTRIB,REAL_MUL_LID] >> `(0:real)<2` by fs[] >>
-    `&TBL2N j * 2 rpow  -&LENGTH j * 2 rpow &LENGTH j <
-     (&TBL2N i +1)  * 2 rpow -&LENGTH i  * 2 rpow &LENGTH j` by
-       metis_tac[RPOW_POS_LT,REAL_LT_RMUL] >>
-    fs[GSYM REAL_MUL_ASSOC,GSYM RPOW_ADD,RPOW_0,add_ints] >> rfs[] >>
-    qabbrev_tac`D=LENGTH j − LENGTH i` >> qabbrev_tac`ii= TBL2N i` >>
-    qabbrev_tac`jj= TBL2N j` >> fs[GSYM GEN_RPOW,REAL_OF_NUM_POW] >>
-    fs[disjoint_pf_lem1])
->- (fs[prefix_free_def,PULL_EXISTS] >>rw[] >>
-  strip_tac >>`interval_bl a <> interval_bl b` by
-   (fs[interval_bl_def] >> rw[] >> `LENGTH a < LENGTH b` by simp[prefix_length_lt]>>
-    `real_of_num (LENGTH a) < real_of_num (LENGTH b)` by fs[REAL_LT] >>
-    `-(real_of_num (LENGTH b)) < -(real_of_num(LENGTH a))` by fs[REAL_LT_NEG] >>
-    `1<(2:real)` by simp[]>>`2 rpow -&LENGTH b < 2 rpow -&LENGTH a` by fs[RPOW_LT]>>
-    fs[REAL_LT_IMP_NE])>>
-  first_x_assum drule_all >>
-  fs[interval_bl_def,disjoint_interval_def] >> rw[DISJOINT_DEF,EXTENSION] >>
-  qexists_tac`&TBL2N b * 2 rpow -&LENGTH b` >> rw[]
-    >- (`0<2 rpow &LENGTH b` by fs[RPOW_POS_LT] >>
-        drule_then (ONCE_REWRITE_TAC o list_of_singleton o GSYM) REAL_LE_RMUL >>
-        fs[GSYM REAL_MUL_ASSOC,GSYM RPOW_ADD,RPOW_0,add_ints]>>
-        drule_then assume_tac prefix_length_lt >> simp[] >>
-        fs[GSYM GEN_RPOW,REAL_OF_NUM_POW] >> fs[prefix_append,TBL2N_append]  )
-    >- (`0<2 rpow &LENGTH b` by fs[RPOW_POS_LT] >>
-        drule_then (ONCE_REWRITE_TAC o list_of_singleton o GSYM) REAL_LT_RMUL >>
-        drule_then assume_tac prefix_length_lt >>
-        fs[GSYM REAL_MUL_ASSOC,GSYM RPOW_ADD,RPOW_0,add_ints,
-           REAL_ADD_RDISTRIB,GSYM GEN_RPOW,REAL_OF_NUM_POW] >>
-        fs[prefix_append,TBL2N_append] )
-    >- (rw[REAL_LT_ADDR] >> `0<(2:real)` by simp[] >> fs[RPOW_POS_LT]) ))
-
-
-val size_of_interval_bl = Q.store_thm("size_of_interval_bl",
-`Normal (SND (interval_bl y))  = Normal (2 rpow -&LENGTH y)`,
-rw[interval_bl_def])
-
-val TBL2N_append_sing_ub = Q.store_thm("TBL2N_append_sing_ub",
-`&(TBL2N (a++[h]) + 1)*2 rpow (-1) <= &(TBL2N a + 1)`,
-`&(2 * TBL2N a + 2) * 2 rpow -1 <= &(TBL2N a + 1)` by
-  (`&(2 * TBL2N a + 2) * 2 rpow -1 = &(2*(TBL2N a + 1)) * 2 rpow -1` by fs[GSYM LEFT_ADD_DISTRIB]>>
-   `_ = 2 * &(TBL2N a + 1) * 2 rpow -1` by fs[REAL_MUL] >>
-   `_ = &(TBL2N a + 1)*(2 rpow 1 * 2 rpow -1)`by
-     fs[AC REAL_MUL_ASSOC REAL_MUL_COMM,RPOW_1]>>
-   `_ = &(TBL2N a + 1) * 2 rpow (1+ -1)` by fs[RPOW_ADD] >>
-   fs[RPOW_0,REAL_ADD_RINV]  ) >>
-Cases_on`h` >> rw[TBL2N_append] >>
-`&(2 * TBL2N a + 1) * 2 rpow -1 <= &(2 * TBL2N a + 2) * 2 rpow -1` by
-  (irule REAL_LE_RMUL_IMP >> rw[RPOW_POS_LT,REAL_LE_LT]) >>
-irule REAL_LE_TRANS >> qexists_tac`&(2 * TBL2N a + 2) * 2 rpow -1` >> rw[] )
-
-val interval_bl_bounds = Q.store_thm("interval_bl_bounds",
-`0<= FST (interval_bl a) /\ FST (interval_bl a) + SND (interval_bl a) <= 1`,
-rw[] >- (fs[interval_bl_def] >> `(0:real)<= &TBL2N a` by fs[tbl2n_def] >> `(0:real)<2` by simp[] >>
-         `0<2 rpow -&LENGTH a` by fs[RPOW_POS_LT] >>
-         metis_tac[util_probTheory.REAL_LE_LT_MUL] )
-     >- (fs[interval_bl_def] >>
-         `&TBL2N a * 2 rpow -&LENGTH a + 2 rpow -&LENGTH a = (&TBL2N a +1)* 2 rpow -&LENGTH a` by
-         fs[REAL_RDISTRIB] >> pop_assum SUBST1_TAC >>
-         `0<2 rpow &LENGTH a` by fs[RPOW_POS_LT] >>
-        drule_then (ONCE_REWRITE_TAC o list_of_singleton o GSYM) REAL_LE_RMUL >>
-        simp[GSYM REAL_MUL_ASSOC,GSYM RPOW_ADD,RPOW_0,GSYM GEN_RPOW,REAL_OF_NUM_POW] >>
-        (TBL2N_ub |> Q.INST [`l`|->`a`] |> assume_tac) >> simp[]  ) )
-
-val bls_size_def = Define`bls_size (P:bool list -> bool) n = SIGMA (\s. (2 rpow -&LENGTH s)) {x|x IN P /\ LENGTH x < n }`
-
-
-
-val finite_and = Q.store_thm("finite_and",
-`FINITE {s| P s} ==> FINITE {s|  Q s /\ P s}`,
-rw[] >> `{s | Q s /\ P s} = {s | Q s}  INTER {s | P s}` by fs[INTER_DEF] >> fs[FINITE_INTER])
-
-val interval_bl_sigma = Q.store_thm("interval_bl_sigma",
-`FINITE  {x | x IN P} ==>
-SIGMA (\a. SND (interval_bl a)) {x | x IN P} = SIGMA (\a. 2 rpow -&LENGTH a) {x | x IN P} `,
-rw[] >> irule REAL_SUM_IMAGE_EQ >> rw[] >> simp[interval_bl_def]);
-
+Theorem interval_bl_sigma:
+  FINITE  {x | x IN P} ==>
+  SIGMA (\a. SND (interval_bl a)) {x | x IN P} =
+  SIGMA (\a. 2 rpow -&LENGTH a) {x | x IN P}
+Proof
+  rw[] >> irule REAL_SUM_IMAGE_EQ >> rw[] >> simp[interval_bl_def]
+QED
 
 fun fsr thl = full_simp_tac(srw_ss () ++ realSimps.REAL_ARITH_ss) thl;
 
+Theorem disjoint_interval_thm:
+  disjoint_interval (interval_bl i) (interval_bl j) ==>
+  FST (interval_bl i) + SND (interval_bl i) <= FST (interval_bl j) \/
+  FST (interval_bl j) + SND (interval_bl j) <= FST (interval_bl i)
+Proof
+  rw[interval_bl_def,disjoint_interval_def,DISJOINT_DEF,EXTENSION,
+     PULL_EXISTS] >>
+  Cases_on‘&TBL2N i * 2 rpow -&LENGTH i + 2 rpow -&LENGTH i <
+           &TBL2N j * 2 rpow -&LENGTH j’ >>
+  fsr[]>>
+  qabbrev_tac‘id=2 rpow -&LENGTH i’ >> qmatch_abbrev_tac‘_ \/ jj+jd<=ii:real’ >>
+  spose_not_then assume_tac >>
+  fsr[REAL_NOT_LT,REAL_NOT_LE]  >>
+  first_x_assum(fn th => qspec_then‘jj’ assume_tac th >>
+                qspec_then‘ii’ assume_tac th) >> fsr[]
+  >- (‘id<= 0’ by metis_tac[REAL_LE_LADD,REAL_ADD_RID] >>
+      ‘0<id’ suffices_by metis_tac[REAL_LET_TRANS,REAL_LT_REFL] >>
+      simp[Abbr‘id’,RPOW_POS_LT])
+  >- (‘jd<= 0’ by metis_tac[REAL_LE_LADD,REAL_ADD_RID] >>
+      ‘0<jd’ suffices_by metis_tac[REAL_LET_TRANS,REAL_LT_REFL] >>
+      simp[Abbr‘jd’,RPOW_POS_LT])
+QED
 
+Triviality max_rs_lemma:
+  !s. FINITE s ==> s<>{} ==> ?x:real. x IN s /\ !y. y IN s ==> y<=x
+Proof
+  Induct_on‘FINITE’ >>rw[] >> Cases_on‘s={}’ >> fs[] >> qexists_tac‘max e x’ >>
+  fsr[max_def] >> rw[]
+  >- metis_tac[] >> Cases_on‘y=e’>> fsr[] >> RES_TAC >> fsr[]
+QED
 
-val disjoint_interval_thm = Q.store_thm("disjoint_interval_thm",
-`disjoint_interval (interval_bl i) (interval_bl j) ==>
-FST (interval_bl i) + SND (interval_bl i) <= FST (interval_bl j) \/
-FST (interval_bl j) + SND (interval_bl j) <= FST (interval_bl i)`,
-rw[interval_bl_def,disjoint_interval_def,DISJOINT_DEF,EXTENSION,PULL_EXISTS] >>
-Cases_on` &TBL2N i * 2 rpow -&LENGTH i + 2 rpow -&LENGTH i < &TBL2N j * 2 rpow -&LENGTH j` >>
-fsr[]>>
-qabbrev_tac`id=2 rpow -&LENGTH i` >> qmatch_abbrev_tac`_ \/ jj+jd<=ii:real` >>
-spose_not_then assume_tac >>
-fsr[REAL_NOT_LT,REAL_NOT_LE]  >>
-first_x_assum(fn th => qspec_then`jj` assume_tac th >> qspec_then`ii` assume_tac th) >> fsr[]
->- (`id<= 0` by metis_tac[REAL_LE_LADD,REAL_ADD_RID] >>
-    `0<id` suffices_by metis_tac[REAL_LET_TRANS,REAL_LT_REFL] >> simp[Abbr`id`,RPOW_POS_LT])
->- (`jd<= 0` by metis_tac[REAL_LE_LADD,REAL_ADD_RID] >>
-    `0<jd` suffices_by metis_tac[REAL_LET_TRANS,REAL_LT_REFL] >> simp[Abbr`jd`,RPOW_POS_LT]) )
+Triviality min_rs_lemma:
+  !s. FINITE s ==> s<>{} ==> ?x:real. x IN s /\ !y. y IN s ==> x<=y
+Proof
+  Induct_on‘FINITE’ >>rw[] >> Cases_on‘s={}’ >> fs[] >> qexists_tac‘min e x’ >>
+  fsr[min_def] >> rw[]>>
+  Cases_on‘y=e’>> fsr[] >> RES_TAC >> fsr[]
+QED
 
+Theorem maxr_set_def = new_specification(
+  "maxr_set_def",["maxr_set"],
+  SIMP_RULE(srw_ss() )[SKOLEM_THM,GSYM RIGHT_EXISTS_IMP_THM] max_rs_lemma
+  );
 
-val max_rs_lemma = Q.prove(`!s. FINITE s ==> s<>{} ==> ?x:real. x IN s /\ !y. y IN s ==> y<=x`,
-Induct_on`FINITE` >>rw[] >> Cases_on`s={}` >> fs[] >> qexists_tac`max e x` >> fsr[max_def] >> rw[]
->- metis_tac[] >> Cases_on`y=e`>> fsr[] >> RES_TAC >> fsr[] )
+Theorem minr_set_def = new_specification(
+  "minr_set_def",["minr_set"],
+  SIMP_RULE(srw_ss() )[SKOLEM_THM,GSYM RIGHT_EXISTS_IMP_THM] min_rs_lemma);
 
-val min_rs_lemma = Q.prove(`!s. FINITE s ==> s<>{} ==> ?x:real. x IN s /\ !y. y IN s ==> x<=y`,
-Induct_on`FINITE` >>rw[] >> Cases_on`s={}` >> fs[] >> qexists_tac`min e x` >> fsr[min_def] >> rw[]>>
-Cases_on`y=e`>> fsr[] >> RES_TAC >> fsr[] )
-
-val maxr_set_def = new_specification("maxr_set_def",["maxr_set"],
-SIMP_RULE(srw_ss() )[SKOLEM_THM,GSYM RIGHT_EXISTS_IMP_THM] max_rs_lemma)
-
-val minr_set_def = new_specification("minr_set_def",["minr_set"],
-SIMP_RULE(srw_ss() )[SKOLEM_THM,GSYM RIGHT_EXISTS_IMP_THM] min_rs_lemma)
-
-val exten_def = Define`exten s = (minr_set {FST k| k IN s},maxr_set {FST k + SND k|k IN s})`
+Definition exten_def:
+  exten s = (minr_set {FST k| k IN s},maxr_set {FST k + SND k|k IN s})
+End
 
 val maxr_set_thm = Q.store_thm("maxr_set_thm[simp]",
-`maxr_set {e} = e /\ (FINITE s /\ s<> {} ==> maxr_set (e INSERT s) = max e (maxr_set s))`,
-rw[] >- (qspec_then `{e}` mp_tac maxr_set_def >> simp[]) >>
-qspec_then `e INSERT s` mp_tac maxr_set_def  >> simp[] >> strip_tac >>
-qabbrev_tac`m = maxr_set (e INSERT s)` >> qspec_then`s` mp_tac maxr_set_def >> simp[] >>
-qabbrev_tac`m0 = maxr_set s` >> rw[] >> rw[max_def]
->- (Cases_on`e = m0` >> rw[] >- (simp[Abbr`m`,ABSORPTION_RWT]) >> Cases_on`e=m` >> rw[]
-    >- (`m0<=e` by metis_tac[] >> fsr[]) >> metis_tac[REAL_LE_ANTISYM]  ) >>
-spose_not_then strip_assume_tac >> `m<=m0` by fsr[] >> `m<e` by fsr[] >> `e<=m` by fsr[] >> fsr[])
+‘maxr_set {e} = e /\ (FINITE s /\ s<> {} ==> maxr_set (e INSERT s) = max e (maxr_set s))’,
+rw[] >- (qspec_then ‘{e}’ mp_tac maxr_set_def >> simp[]) >>
+qspec_then ‘e INSERT s’ mp_tac maxr_set_def  >> simp[] >> strip_tac >>
+qabbrev_tac‘m = maxr_set (e INSERT s)’ >> qspec_then‘s’ mp_tac maxr_set_def >> simp[] >>
+qabbrev_tac‘m0 = maxr_set s’ >> rw[] >> rw[max_def]
+>- (Cases_on‘e = m0’ >> rw[] >- (simp[Abbr‘m’,ABSORPTION_RWT]) >> Cases_on‘e=m’ >> rw[]
+    >- (‘m0<=e’ by metis_tac[] >> fsr[]) >> metis_tac[REAL_LE_ANTISYM]  ) >>
+spose_not_then strip_assume_tac >> ‘m<=m0’ by fsr[] >> ‘m<e’ by fsr[] >> ‘e<=m’ by fsr[] >> fsr[])
 
 val minr_set_thm = Q.store_thm("minr_set_thm[simp]",
-`minr_set {e} = e /\ (FINITE s /\ s<> {} ==> minr_set (e INSERT s) = min e (minr_set s))`,
-rw[] >- (qspec_then `{e}` mp_tac minr_set_def >> simp[]) >>
-qspec_then `e INSERT s` mp_tac minr_set_def  >> simp[] >> strip_tac >>
-qabbrev_tac`m = minr_set (e INSERT s)` >> qspec_then`s` mp_tac minr_set_def >> simp[] >>
-qabbrev_tac`m0 = minr_set s` >> rw[] >> rw[min_def]
->- (Cases_on`e = m0` >> rw[] >- (simp[Abbr`m`,ABSORPTION_RWT]) >> Cases_on`e=m` >> rw[] >>
-    `m<=e` by metis_tac[] >>`m IN s` by fs[] >>`m0<=m` by fs[] >> metis_tac[REAL_LE_ANTISYM]) >>
-spose_not_then strip_assume_tac >> `m<=m0` by fsr[] >> `m0<e` by fsr[] >> `m<=e` by fsr[] >>
-Cases_on`m=e` >> fsr[] >> `m0 <= m` by fsr[] >> fsr[])
+‘minr_set {e} = e /\ (FINITE s /\ s<> {} ==> minr_set (e INSERT s) = min e (minr_set s))’,
+rw[] >- (qspec_then ‘{e}’ mp_tac minr_set_def >> simp[]) >>
+qspec_then ‘e INSERT s’ mp_tac minr_set_def  >> simp[] >> strip_tac >>
+qabbrev_tac‘m = minr_set (e INSERT s)’ >> qspec_then‘s’ mp_tac minr_set_def >> simp[] >>
+qabbrev_tac‘m0 = minr_set s’ >> rw[] >> rw[min_def]
+>- (Cases_on‘e = m0’ >> rw[] >- (simp[Abbr‘m’,ABSORPTION_RWT]) >> Cases_on‘e=m’ >> rw[] >>
+    ‘m<=e’ by metis_tac[] >>‘m IN s’ by fs[] >>‘m0<=m’ by fs[] >> metis_tac[REAL_LE_ANTISYM]) >>
+spose_not_then strip_assume_tac >> ‘m<=m0’ by fsr[] >> ‘m0<e’ by fsr[] >> ‘m<=e’ by fsr[] >>
+Cases_on‘m=e’ >> fsr[] >> ‘m0 <= m’ by fsr[] >> fsr[])
 
 val maxr_set_union = Q.store_thm("maxr_set_union",
-`!s1. (FINITE s1) ==> !s2. (FINITE s2) ==> (s1 <> EMPTY /\  s2 <> EMPTY ) ==>
-  maxr_set (s1 UNION s2)=max (maxr_set s1) (maxr_set s2)`,
-Induct_on`FINITE` >> strip_tac
->- (Induct_on`FINITE` >>rw[maxr_set_thm] )
->- (ntac 4 strip_tac >> Induct_on`FINITE` >> rw[maxr_set_thm] >>
-    Cases_on`s2 <> {}` >> Cases_on`s1 <> {}` >> rw[] >>simp[maxr_set_thm]
-    >- (Cases_on`e<= maxr_set s1` >> Cases_on`e'<= maxr_set s2` >>
+‘!s1. (FINITE s1) ==> !s2. (FINITE s2) ==> (s1 <> EMPTY /\  s2 <> EMPTY ) ==>
+  maxr_set (s1 UNION s2)=max (maxr_set s1) (maxr_set s2)’,
+Induct_on‘FINITE’ >> strip_tac
+>- (Induct_on‘FINITE’ >>rw[maxr_set_thm] )
+>- (ntac 4 strip_tac >> Induct_on‘FINITE’ >> rw[maxr_set_thm] >>
+    Cases_on‘s2 <> {}’ >> Cases_on‘s1 <> {}’ >> rw[] >>simp[maxr_set_thm]
+    >- (Cases_on‘e<= maxr_set s1’ >> Cases_on‘e'<= maxr_set s2’ >>
         fs[max_def,maxr_set_thm,INSERT_UNION_EQ] >> rw[] >> fsr[]
-        >- (Cases_on`maxr_set s1 <= maxr_set s2` >> fsr[])
-        >- (Cases_on`maxr_set s1 <= e'` >> fsr[]) )
-    >- (Cases_on`e'<= maxr_set s2` >>
+        >- (Cases_on‘maxr_set s1 <= maxr_set s2’ >> fsr[])
+        >- (Cases_on‘maxr_set s1 <= e'’ >> fsr[]) )
+    >- (Cases_on‘e'<= maxr_set s2’ >>
         fs[max_def,maxr_set_thm,INSERT_UNION_EQ] >> rw[] >> fsr[])
-    >- (Cases_on`e<= maxr_set s1` >> fs[max_def,maxr_set_thm,INSERT_UNION_EQ] >> rw[] >>
-        fsr[] >> Cases_on`maxr_set s1 <= e'` >> fsr[])
+    >- (Cases_on‘e<= maxr_set s1’ >> fs[max_def,maxr_set_thm,INSERT_UNION_EQ] >> rw[] >>
+        fsr[] >> Cases_on‘maxr_set s1 <= e'’ >> fsr[])
     >- (fs[max_def,maxr_set_thm,INSERT_UNION_EQ]) )
 )
 
 
 val minr_set_union = Q.store_thm("minr_set_union",
-`!s1. (FINITE s1) ==> !s2. (FINITE s2) ==> (s1 <> EMPTY /\  s2 <> EMPTY ) ==>
-  minr_set (s1 UNION s2)=min (minr_set s1) (minr_set s2)`,
-Induct_on`FINITE` >> strip_tac
->- (Induct_on`FINITE` >>rw[minr_set_thm] )
->- (ntac 4 strip_tac >> Induct_on`FINITE` >> rw[minr_set_thm] >>
-    Cases_on`s2 <> {}` >> Cases_on`s1 <> {}` >> rw[] >>simp[minr_set_thm]
-    >- (Cases_on`e<= minr_set s1` >> Cases_on`e'<= minr_set s2` >>
+‘!s1. (FINITE s1) ==> !s2. (FINITE s2) ==> (s1 <> EMPTY /\  s2 <> EMPTY ) ==>
+  minr_set (s1 UNION s2)=min (minr_set s1) (minr_set s2)’,
+Induct_on‘FINITE’ >> strip_tac
+>- (Induct_on‘FINITE’ >>rw[minr_set_thm] )
+>- (ntac 4 strip_tac >> Induct_on‘FINITE’ >> rw[minr_set_thm] >>
+    Cases_on‘s2 <> {}’ >> Cases_on‘s1 <> {}’ >> rw[] >>simp[minr_set_thm]
+    >- (Cases_on‘e<= minr_set s1’ >> Cases_on‘e'<= minr_set s2’ >>
         fs[min_def,minr_set_thm,INSERT_UNION_EQ] >> rw[] >> fsr[]
-        >- (Cases_on`minr_set s1 <= e'` >> fsr[])
-        >- (Cases_on`minr_set s1 <= minr_set s2` >> fsr[]) )
-    >- (Cases_on`e<= minr_set s1` >> fs[min_def,minr_set_thm,INSERT_UNION_EQ] >> rw[] >>
-        fsr[] >> Cases_on`minr_set s1 <= e'` >> fsr[])
-    >- (Cases_on`e<= minr_set s1` >> fs[min_def,minr_set_thm,INSERT_UNION_EQ] >> rw[] >>
-        fsr[] >> Cases_on` minr_set s1 <= e'` >>rw[] >> fsr[])
+        >- (Cases_on‘minr_set s1 <= e'’ >> fsr[])
+        >- (Cases_on‘minr_set s1 <= minr_set s2’ >> fsr[]) )
+    >- (Cases_on‘e<= minr_set s1’ >> fs[min_def,minr_set_thm,INSERT_UNION_EQ] >> rw[] >>
+        fsr[] >> Cases_on‘minr_set s1 <= e'’ >> fsr[])
+    >- (Cases_on‘e<= minr_set s1’ >> fs[min_def,minr_set_thm,INSERT_UNION_EQ] >> rw[] >>
+        fsr[] >> Cases_on‘ minr_set s1 <= e'’ >>rw[] >> fsr[])
     >- (fs[min_def,minr_set_thm,INSERT_UNION_EQ]) )
 )
 
 
 val gspec_eq = Q.store_thm("gspec_eq[simp]",
-`GSPEC (\x. (f x,x=k)) = {f k}`,
+‘GSPEC (\x. (f x,x=k)) = {f k}’,
 simp[EXTENSION])
 
 val gspec_in = Q.store_thm("gspec_in[simp]",
-`GSPEC (\x. (f x,x IN k)) = {f x|x IN k}`,
+‘GSPEC (\x. (f x,x IN k)) = {f x|x IN k}’,
 simp[EXTENSION])
 
 val gspec_f_or = Q.store_thm("gspec_f_or[simp]",
-`!P Q. {f x | P x \/ Q x} = {f x | P x} UNION {f x | Q x}`,
+‘!P Q. {f x | P x \/ Q x} = {f x | P x} UNION {f x | Q x}’,
 rw[IN_UNION,EXTENSION] >> metis_tac[GSPECIFICATION_applied])
 
 
 
 val exten_insert_thm = Q.store_thm("exten_insert_thm",
-`(s <> EMPTY /\ FINITE s) ==> exten (e INSERT s) =  (min (FST e) ## max (FST e + SND e)) (exten s)`,
+‘(s <> EMPTY /\ FINITE s) ==> exten (e INSERT s) =  (min (FST e) ## max (FST e + SND e)) (exten s)’,
 simp[exten_def,maxr_set_thm,minr_set_thm] >> rw[]
->- (`{FST k | k <> e ==> k IN s} = {FST k | k = e \/ k IN s}` by fs[EXTENSION] >>
-    `{FST k | k = e \/ k IN s} = {FST k | k = e} UNION {FST k | k IN s}` by fs[] >> rw[] >>
-    `FINITE {FST e}` by fs[] >> `{FST e} <> {}` by fs[] >>
-    `FINITE {FST k | k IN s}` by metis_tac[IMAGE_FINITE,IMAGE_DEF] >>
-    `{FST k | k IN s} <> {}` by metis_tac[IMAGE_EQ_EMPTY,IMAGE_DEF]>>
+>- (‘{FST k | k <> e ==> k IN s} = {FST k | k = e \/ k IN s}’ by fs[EXTENSION] >>
+    ‘{FST k | k = e \/ k IN s} = {FST k | k = e} UNION {FST k | k IN s}’ by fs[] >> rw[] >>
+    ‘FINITE {FST e}’ by fs[] >> ‘{FST e} <> {}’ by fs[] >>
+    ‘FINITE {FST k | k IN s}’ by metis_tac[IMAGE_FINITE,IMAGE_DEF] >>
+    ‘{FST k | k IN s} <> {}’ by metis_tac[IMAGE_EQ_EMPTY,IMAGE_DEF]>>
     rw[minr_set_union])
->- (`{FST k + SND k | k <> e ==> k IN s} = {FST k + SND k | k = e \/ k IN s}` by fs[EXTENSION] >>
-    `{FST k + SND k | k = e \/ k IN s} = {FST k + SND k | k = e} UNION {FST k + SND k | k IN s}` by fs[] >>
+>- (‘{FST k + SND k | k <> e ==> k IN s} = {FST k + SND k | k = e \/ k IN s}’ by fs[EXTENSION] >>
+    ‘{FST k + SND k | k = e \/ k IN s} = {FST k + SND k | k = e} UNION {FST k + SND k | k IN s}’ by fs[] >>
     rw[] >>
-    `FINITE {FST e  + SND k}` by fs[] >> `{FST e  + SND k} <> {}` by fs[] >>
-    `FINITE {FST k + SND k | k IN s}` by metis_tac[IMAGE_FINITE,IMAGE_DEF] >>
-    `{FST k + SND k | k IN s} <> {}` by metis_tac[IMAGE_EQ_EMPTY,IMAGE_DEF]>>
+    ‘FINITE {FST e  + SND k}’ by fs[] >> ‘{FST e  + SND k} <> {}’ by fs[] >>
+    ‘FINITE {FST k + SND k | k IN s}’ by metis_tac[IMAGE_FINITE,IMAGE_DEF] >>
+    ‘{FST k + SND k | k IN s} <> {}’ by metis_tac[IMAGE_EQ_EMPTY,IMAGE_DEF]>>
     rw[maxr_set_union] ))
 
 val TBL2N_ub2 = Q.store_thm("TBL2N_ub2",
-`&TBL2N x * 2 rpow -&LENGTH x +  2 rpow -&LENGTH x <= 1`,
-`0<2 rpow &LENGTH x` by fs[RPOW_POS_LT] >>
+‘&TBL2N x * 2 rpow -&LENGTH x +  2 rpow -&LENGTH x <= 1’,
+‘0<2 rpow &LENGTH x’ by fs[RPOW_POS_LT] >>
 drule_then (ONCE_REWRITE_TAC o list_of_singleton o GSYM) REAL_LE_RMUL >>
 simp[REAL_ADD_RDISTRIB,GSYM REAL_MUL_ASSOC,GSYM RPOW_ADD,RPOW_0,GSYM GEN_RPOW,REAL_OF_NUM_POW] >>
-(TBL2N_ub |> Q.INST [`l`|->`x`] |> assume_tac) >> simp[TBL2N_ub] )
+(TBL2N_ub |> Q.INST [‘l’|->‘x’] |> assume_tac) >> simp[TBL2N_ub] )
 
 val rpow_len_lb = Q.store_thm("rpow_len_lb",
-`0<  2 rpow -&LENGTH x`,
+‘0<  2 rpow -&LENGTH x’,
 fs[RPOW_POS_LT])
 
 val TBL2N_lb = Q.store_thm("TBL2N_lb",
-`0<= &TBL2N x * 2 rpow -&LENGTH x`,
-`0<2 rpow &LENGTH x` by fs[RPOW_POS_LT] >>
+‘0<= &TBL2N x * 2 rpow -&LENGTH x’,
+‘0<2 rpow &LENGTH x’ by fs[RPOW_POS_LT] >>
 drule_then (ONCE_REWRITE_TAC o list_of_singleton o GSYM) REAL_LE_RMUL >>
 simp[REAL_ADD_RDISTRIB,GSYM REAL_MUL_ASSOC,GSYM RPOW_ADD,RPOW_0,GSYM GEN_RPOW,REAL_OF_NUM_POW])
 
 val lemma11 = Q.store_thm("lemma11",
-`!s. FINITE s ==> (!x dx y dy. (x,dx) IN s /\ (y,dy) IN s /\ x<>y ==> x+dx<=y \/ y+dy<=x) /\
+‘!s. FINITE s ==> (!x dx y dy. (x,dx) IN s /\ (y,dy) IN s /\ x<>y ==> x+dx<=y \/ y+dy<=x) /\
               (!x d. (x,d) IN s ==> 0r<d) /\ (!x d. (x,d) IN s ==> 0<= x /\ x+d <=1) /\ (s <> {})
-          ==> (0<= FST (exten s) /\ SND (exten s) <= 1)`,
-Induct_on`FINITE` >> simp[] >>ntac 2 (gen_tac>>strip_tac) >>strip_tac >> Cases_on`s={}` >> fs[]
->- (simp[maxr_set_def,minr_set_def,exten_def,ITSET_THM] >> Cases_on`e` >> fs[]) >>
+          ==> (0<= FST (exten s) /\ SND (exten s) <= 1)’,
+Induct_on‘FINITE’ >> simp[] >>ntac 2 (gen_tac>>strip_tac) >>strip_tac >> Cases_on‘s={}’ >> fs[]
+>- (simp[maxr_set_def,minr_set_def,exten_def,ITSET_THM] >> Cases_on‘e’ >> fs[]) >>
 fs[exten_insert_thm] >> rw[max_def,min_def]
->- (Cases_on`e` >> fsr[] >> metis_tac[])
+>- (Cases_on‘e’ >> fsr[] >> metis_tac[])
 >- (metis_tac[])
 >- (metis_tac[]) )
 
 
 
 val BETTER_RPOW_UNIQ_EXP = Q.store_thm("BETTER_RPOW_UNIQ_EXP[simp]",
-`1r < a ==> (a rpow b = a rpow c <=> b = c)`,
-rw[] >> eq_tac >> simp[] >> rw[] >> pop_assum (mp_tac o AP_TERM ``transc$ln``) >> fsr[LN_RPOW] >>
-disch_then irule >> `ln 1 < ln a` by fsr[LN_MONO_LT] >> fsr[LN_1] )
+‘1r < a ==> (a rpow b = a rpow c <=> b = c)’,
+rw[] >> eq_tac >> simp[] >> rw[] >> pop_assum (mp_tac o AP_TERM “transc$ln”) >> fsr[LN_RPOW] >>
+disch_then irule >> ‘ln 1 < ln a’ by fsr[LN_MONO_LT] >> fsr[LN_1] )
 
 
 val interval_bl_11 = Q.store_thm("interval_bl_11[simp]",
-`interval_bl x = interval_bl y <=> x = y`,
+‘interval_bl x = interval_bl y <=> x = y’,
 simp[interval_bl_def] >> eq_tac >> simp[] >> rw[] >> fsr[TBL2N_inj_len,RPOW_NZ])
 
 val interval_bl_inj = Q.store_thm("interval_bl_inj",
-`INJ interval_bl P (IMAGE interval_bl P)`,
+‘INJ interval_bl P (IMAGE interval_bl P)’,
 simp[INJ_DEF])
 
-val lemma12 = Q.prove(`bls_size P n = SIGMA SND (IMAGE interval_bl {s|s IN P /\ LENGTH s < n})`,
+val lemma12 = Q.prove(‘bls_size P n = SIGMA SND (IMAGE interval_bl {s|s IN P /\ LENGTH s < n})’,
 fs[bls_size_def,interval_bl_def,REAL_SUM_IMAGE_IMAGE,interval_bl_inj,finite_bool_list_lt_n,finite_and,combinTheory.o_DEF])
 
 val exten_sing = Q.store_thm("exten_sing[simp]",
-`exten {e} = (FST e,FST e + SND e)`,
+‘exten {e} = (FST e,FST e + SND e)’,
 fs[exten_def])
 
 val size_of_exten = Q.prove(
-`!s. FINITE s ==> (!x dx y dy. (x,dx) IN s /\ (y,dy) IN s /\ (x,dx)<>(y,dy) ==> x+dx<=y \/ y+dy<=x) /\
+‘!s. FINITE s ==> (!x dx y dy. (x,dx) IN s /\ (y,dy) IN s /\ (x,dx)<>(y,dy) ==> x+dx<=y \/ y+dy<=x) /\
               (!x d. (x,d) IN s ==> 0r<d) /\ (s <> {})
-          ==> SIGMA SND s <= SND (exten s) - FST (exten s)`,
+          ==> SIGMA SND s <= SND (exten s) - FST (exten s)’,
 HO_MATCH_MP_TAC FINITE_COMPLETE_INDUCTION >> rw[] >>
-map_every qabbrev_tac[`Rs = {FST k + SND k | k IN s}`,`Ls = {FST k |k IN s}`]>>
-`FINITE Ls` by metis_tac[IMAGE_FINITE,IMAGE_DEF] >>
-`Ls <> {}` by metis_tac[IMAGE_EQ_EMPTY,IMAGE_DEF] >>
-`?e1 e2. (e1,e2) IN s /\ !m. m IN Ls ==> e1<=m`
-  by (qexists_tac `minr_set Ls` >> qexists_tac`@e'. (minr_set Ls,e') IN s` >> reverse(rw[])
+map_every qabbrev_tac[‘Rs = {FST k + SND k | k IN s}’,‘Ls = {FST k |k IN s}’]>>
+‘FINITE Ls’ by metis_tac[IMAGE_FINITE,IMAGE_DEF] >>
+‘Ls <> {}’ by metis_tac[IMAGE_EQ_EMPTY,IMAGE_DEF] >>
+‘?e1 e2. (e1,e2) IN s /\ !m. m IN Ls ==> e1<=m’
+  by (qexists_tac ‘minr_set Ls’ >> qexists_tac‘@e'. (minr_set Ls,e') IN s’ >> reverse(rw[])
       >- (metis_tac[minr_set_def]) >> SELECT_ELIM_TAC >> simp[] >>
-      `minr_set Ls IN Ls` by metis_tac[minr_set_def] >> fs[Abbr`Ls`] >>
+      ‘minr_set Ls IN Ls’ by metis_tac[minr_set_def] >> fs[Abbr‘Ls’] >>
       metis_tac[pairTheory.PAIR]) >>
-qabbrev_tac`s0 = s DELETE (e1,e2)` >> Cases_on`s0={}` >> simp[]
-  >- (`s = {(e1,e2)}` by (metis_tac[DELETE_EQ_SING]) >> rw[REAL_SUM_IMAGE_THM] >> fsr[]) >>
-`s0 ⊂ s` by (fs[Abbr`s0`,PSUBSET_MEMBER]>> metis_tac[]) >> last_x_assum drule >> impl_tac
-  >- (rw[Abbr`s0`] >> metis_tac[]) >> `s = (e1,e2) INSERT s0` by fs[Abbr`s0`] >>
-`s0 DELETE (e1,e2) = s0` by fs[Abbr`s0`,ELT_IN_DELETE,DELETE_NON_ELEMENT] >>
+qabbrev_tac‘s0 = s DELETE (e1,e2)’ >> Cases_on‘s0={}’ >> simp[]
+  >- (‘s = {(e1,e2)}’ by (metis_tac[DELETE_EQ_SING]) >> rw[REAL_SUM_IMAGE_THM] >> fsr[]) >>
+‘s0 ⊂ s’ by (fs[Abbr‘s0’,PSUBSET_MEMBER]>> metis_tac[]) >> last_x_assum drule >> impl_tac
+  >- (rw[Abbr‘s0’] >> metis_tac[]) >> ‘s = (e1,e2) INSERT s0’ by fs[Abbr‘s0’] >>
+‘s0 DELETE (e1,e2) = s0’ by fs[Abbr‘s0’,ELT_IN_DELETE,DELETE_NON_ELEMENT] >>
 fsr[REAL_SUM_IMAGE_THM] >>
-`SND (exten s0) - FST (exten s0) <=  SND (exten ((e1,e2) INSERT s0)) − FST (exten ((e1,e2) INSERT s0)) - e2` suffices_by fsr[] >>
+‘SND (exten s0) - FST (exten s0) <=  SND (exten ((e1,e2) INSERT s0)) − FST (exten ((e1,e2) INSERT s0)) - e2’ suffices_by fsr[] >>
 fsr[exten_def,exten_insert_thm,REAL_SUM_IMAGE_THM,DELETE_NON_ELEMENT_RWT] >>
-map_every qabbrev_tac [`MX = maxr_set {FST k + SND k | k IN s0}`,`MN = minr_set  {FST k | k IN s0}`]>>
-map_every qabbrev_tac[`Rs0 = {FST k + SND k | k IN s0}`,`Ls0 = {FST k |k IN s0}`] >>
-`FINITE Ls0` by metis_tac[IMAGE_FINITE,IMAGE_DEF] >>
-`Ls0 <> {}` by metis_tac[IMAGE_EQ_EMPTY,IMAGE_DEF] >>
-`MN IN Ls0` by metis_tac[minr_set_def] >>
-`?n. (MN,n) IN s0` by (`?p. p IN s0 /\ FST p = MN` suffices_by (rw[] >> metis_tac[pairTheory.PAIR]) >>
-                    pop_assum MP_TAC >> simp[Abbr`Ls0`] >> metis_tac[]) >>
-`MN IN Ls` by (simp[Abbr`Ls`] >>metis_tac[pairTheory.FST]) >>
+map_every qabbrev_tac [‘MX = maxr_set {FST k + SND k | k IN s0}’,‘MN = minr_set  {FST k | k IN s0}’]>>
+map_every qabbrev_tac[‘Rs0 = {FST k + SND k | k IN s0}’,‘Ls0 = {FST k |k IN s0}’] >>
+‘FINITE Ls0’ by metis_tac[IMAGE_FINITE,IMAGE_DEF] >>
+‘Ls0 <> {}’ by metis_tac[IMAGE_EQ_EMPTY,IMAGE_DEF] >>
+‘MN IN Ls0’ by metis_tac[minr_set_def] >>
+‘?n. (MN,n) IN s0’ by (‘?p. p IN s0 /\ FST p = MN’ suffices_by (rw[] >> metis_tac[pairTheory.PAIR]) >>
+                    pop_assum MP_TAC >> simp[Abbr‘Ls0’] >> metis_tac[]) >>
+‘MN IN Ls’ by (simp[Abbr‘Ls’] >>metis_tac[pairTheory.FST]) >>
 rw[max_def,min_def] >> fsr[]
->- (`e1 + e2 <= MN` suffices_by fsr[] >>
-    first_x_assum(qspecl_then[`e1`,`e2`,`MN`,`n`] MP_TAC) >> simp[] >> impl_tac
-    >- (rpt strip_tac >> rw[] >> rw[Abbr`s0`] >> fs[]) >> strip_tac >> `e1<=MN` by fs[]>>
-     `0<n` suffices_by fsr[] >> metis_tac[]  )
->- (`MX < e1+e2` by fsr[] >> `FINITE Rs0` by metis_tac[IMAGE_FINITE,IMAGE_DEF] >>
-    `Rs0 <> {}` by metis_tac[IMAGE_EQ_EMPTY,IMAGE_DEF] >>`MX IN Rs0` by metis_tac[maxr_set_def]>>
-    `?i j. (i,j) IN s0 /\ MX = i+j` by (pop_assum MP_TAC >> simp[Abbr`Rs0`] >>
+>- (‘e1 + e2 <= MN’ suffices_by fsr[] >>
+    first_x_assum(qspecl_then[‘e1’,‘e2’,‘MN’,‘n’] MP_TAC) >> simp[] >> impl_tac
+    >- (rpt strip_tac >> rw[] >> rw[Abbr‘s0’] >> fs[]) >> strip_tac >> ‘e1<=MN’ by fs[]>>
+     ‘0<n’ suffices_by fsr[] >> metis_tac[]  )
+>- (‘MX < e1+e2’ by fsr[] >> ‘FINITE Rs0’ by metis_tac[IMAGE_FINITE,IMAGE_DEF] >>
+    ‘Rs0 <> {}’ by metis_tac[IMAGE_EQ_EMPTY,IMAGE_DEF] >>‘MX IN Rs0’ by metis_tac[maxr_set_def]>>
+    ‘?i j. (i,j) IN s0 /\ MX = i+j’ by (pop_assum MP_TAC >> simp[Abbr‘Rs0’] >>
                                     metis_tac[pairTheory.PAIR]) >>
-    first_x_assum(qspecl_then[`e1`,`e2`,`i`,`j`] MP_TAC) >> simp[] >> impl_tac
-    >- (rpt strip_tac >> rw[] >> rw[Abbr`s0`] >> fs[]) >> strip_tac
-    >- (rw[] >> `0<j` suffices_by fsr[] >> metis_tac[]) >> rw[] >>
-    `i IN Ls` by (simp[Abbr`Ls`,pairTheory.EXISTS_PROD] >>metis_tac[])>> `e1<=i` by simp[]>>
-    `0<j` suffices_by fsr[] >> metis_tac[]  ) )
+    first_x_assum(qspecl_then[‘e1’,‘e2’,‘i’,‘j’] MP_TAC) >> simp[] >> impl_tac
+    >- (rpt strip_tac >> rw[] >> rw[Abbr‘s0’] >> fs[]) >> strip_tac
+    >- (rw[] >> ‘0<j’ suffices_by fsr[] >> metis_tac[]) >> rw[] >>
+    ‘i IN Ls’ by (simp[Abbr‘Ls’,pairTheory.EXISTS_PROD] >>metis_tac[])>> ‘e1<=i’ by simp[]>>
+    ‘0<j’ suffices_by fsr[] >> metis_tac[]  ) )
 
 
 val exten_member = Q.store_thm("exten_member",
-`FINITE s /\ s <> {} /\ exten (s) = (sn,sx) ==>
- (?sn' sx' dx. (sn,sn') IN s /\ (sx',dx) IN s /\ sx'+dx=sx)`,
-simp[exten_def] >> rw[] >> `{FST k|k IN s} = IMAGE FST s` by simp[EXTENSION] >>
-`FINITE {FST k|k IN s} /\ {FST k | k IN s} <> {}` by simp[] >> drule_all minr_set_def >>rw[] >>
-qexists_tac`SND k` >> simp[] >>
-`{FST k + SND k|k IN s} = IMAGE (\k. FST k+ SND k) s` by simp[EXTENSION] >>
-`FINITE {FST k + SND k|k IN s} /\ {FST k + SND k | k IN s} <> {}` by simp[] >> drule_all maxr_set_def >>
-rw[] >> rename[`maxr_set _ = FST kk + SND kk`] >> map_every qexists_tac [`FST kk`,`SND kk`] >> simp[])
+‘FINITE s /\ s <> {} /\ exten (s) = (sn,sx) ==>
+ (?sn' sx' dx. (sn,sn') IN s /\ (sx',dx) IN s /\ sx'+dx=sx)’,
+simp[exten_def] >> rw[] >> ‘{FST k|k IN s} = IMAGE FST s’ by simp[EXTENSION] >>
+‘FINITE {FST k|k IN s} /\ {FST k | k IN s} <> {}’ by simp[] >> drule_all minr_set_def >>rw[] >>
+qexists_tac‘SND k’ >> simp[] >>
+‘{FST k + SND k|k IN s} = IMAGE (\k. FST k+ SND k) s’ by simp[EXTENSION] >>
+‘FINITE {FST k + SND k|k IN s} /\ {FST k + SND k | k IN s} <> {}’ by simp[] >> drule_all maxr_set_def >>
+rw[] >> rename[‘maxr_set _ = FST kk + SND kk’] >> map_every qexists_tac [‘FST kk’,‘SND kk’] >> simp[])
 
-val _ = overload_on ("bpos" ,`` \l. &TBL2N l * 2 rpow -&LENGTH l``);
+val _ = overload_on ("bpos" ,“ \l. &TBL2N l * 2 rpow -&LENGTH l”);
 
 val bpos_min = Q.store_thm("bpos_min",
-`!s. FINITE s ==> s <> {} ==> ?l. l IN s /\ !m. m IN s ==> bpos l <= bpos m`,
-Induct_on`FINITE` >> simp[] >> rw[] >> Cases_on`s={}` >> simp[] >>fs[] >> Cases_on`bpos e <= bpos l`>>
-fs[] >- (qexists_tac`e` >> simp[] >> metis_tac[REAL_LE_TRANS,REAL_LE_REFL]) >> qexists_tac`l` >>
+‘!s. FINITE s ==> s <> {} ==> ?l. l IN s /\ !m. m IN s ==> bpos l <= bpos m’,
+Induct_on‘FINITE’ >> simp[] >> rw[] >> Cases_on‘s={}’ >> simp[] >>fs[] >> Cases_on‘bpos e <= bpos l’>>
+fs[] >- (qexists_tac‘e’ >> simp[] >> metis_tac[REAL_LE_TRANS,REAL_LE_REFL]) >> qexists_tac‘l’ >>
 simp[] >> metis_tac[REAL_NOT_LE,REAL_LT_IMP_LE] )
 
 val exten_low_high = Q.store_thm("exten_low_high",
-`!s. FINITE s ==> s <> {} ==> !low high. exten (IMAGE interval_bl s) = (low,high) ==> low <= high`,
-Induct_on`FINITE` >> simp[] >> rw[] >> Cases_on`s={}` >> simp[] >>fs[]
+‘!s. FINITE s ==> s <> {} ==> !low high. exten (IMAGE interval_bl s) = (low,high) ==> low <= high’,
+Induct_on‘FINITE’ >> simp[] >> rw[] >> Cases_on‘s={}’ >> simp[] >>fs[]
 >- (fs[interval_bl_def] >> rw[REAL_LE_ADDR] >> rw[RPOW_POS_LT,REAL_LE_LT]) >>
-qpat_x_assum`exten _ = _` mp_tac >> rfs[exten_insert_thm] >> Cases_on`exten (IMAGE interval_bl s)` >>
+qpat_x_assum‘exten _ = _’ mp_tac >> rfs[exten_insert_thm] >> Cases_on‘exten (IMAGE interval_bl s)’ >>
 fs[] >> fsr[interval_bl_def,min_def,max_def] >> rw[]>>fsr[] )
 
 
 
-val lemma13 = Q.store_thm("lemma13",`!P. FINITE P ==> (P <> {}) ==>
+val lemma13 = Q.store_thm("lemma13",‘!P. FINITE P ==> (P <> {}) ==>
                            (!x y. x IN P /\ y IN P /\ x <> y ==>
                                   disjoint_interval (interval_bl x) (interval_bl y)) ==>
                            (SIGMA (\s. 2 rpow -&LENGTH s) P + FST (exten (IMAGE interval_bl P) )
-                            <= SND (exten (IMAGE interval_bl P) ))`,
-HO_MATCH_MP_TAC FINITE_COMPLETE_INDUCTION >> rw[] >>qmatch_abbrev_tac`_ <= SND (exten s)` >>
-`?l. l IN P /\ !m. m IN P ==> bpos l <= bpos m` by metis_tac[bpos_min] >>
-qabbrev_tac`P0 = P DELETE l` >> Cases_on`P0={}` >> simp[]
-  >- (`P = {l}` by (metis_tac[DELETE_EQ_SING]) >>
-      fsr[REAL_SUM_IMAGE_THM,Abbr`s`,interval_bl_def,REAL_LE_ADDL,TBL2N_lb]) >>
-`P0⊂ P` by (fs[Abbr`P0`,PSUBSET_MEMBER]>> metis_tac[]) >>  last_x_assum drule >> impl_tac
->- (rw[Abbr`P0`] >> metis_tac[]) >>`P = l INSERT P0` by fs[Abbr`P0`] >>
-`P0 DELETE l = P0` by fs[Abbr`P0`,ELT_IN_DELETE,DELETE_NON_ELEMENT] >>
-fsr[REAL_SUM_IMAGE_THM,Abbr`s`,exten_insert_thm] >>
-`?en ex. exten (IMAGE interval_bl P0) = (en,ex)` by metis_tac[pairTheory.pair_CASES] >> simp[]>>
-`?l0 d. interval_bl l = (l0,d)` by metis_tac[pairTheory.pair_CASES] >> fs[] >>
-`2 rpow -&LENGTH l = d` by fsr[interval_bl_def] >> fs[] >>
-`max (l0 + d) ex = d + max l0 (ex-d)` by (fsr[max_def] >> rw[] >> fsr[]) >>fsr[GSYM REAL_ADD_ASSOC]>>
-`?en'. (en,en') IN IMAGE interval_bl P0` by metis_tac[exten_member,IMAGE_FINITE,IMAGE_EQ_EMPTY]>> fs[]>>
-rename[`(en,en') = interval_bl EN`] >>
-`l0+d<=en` by (first_x_assum (qspecl_then [`l`,`EN`] mp_tac) >>
+                            <= SND (exten (IMAGE interval_bl P) ))’,
+HO_MATCH_MP_TAC FINITE_COMPLETE_INDUCTION >> rw[] >>qmatch_abbrev_tac‘_ <= SND (exten s)’ >>
+‘?l. l IN P /\ !m. m IN P ==> bpos l <= bpos m’ by metis_tac[bpos_min] >>
+qabbrev_tac‘P0 = P DELETE l’ >> Cases_on‘P0={}’ >> simp[]
+  >- (‘P = {l}’ by (metis_tac[DELETE_EQ_SING]) >>
+      fsr[REAL_SUM_IMAGE_THM,Abbr‘s’,interval_bl_def,REAL_LE_ADDL,TBL2N_lb]) >>
+‘P0⊂ P’ by (fs[Abbr‘P0’,PSUBSET_MEMBER]>> metis_tac[]) >>  last_x_assum drule >> impl_tac
+>- (rw[Abbr‘P0’] >> metis_tac[]) >>‘P = l INSERT P0’ by fs[Abbr‘P0’] >>
+‘P0 DELETE l = P0’ by fs[Abbr‘P0’,ELT_IN_DELETE,DELETE_NON_ELEMENT] >>
+fsr[REAL_SUM_IMAGE_THM,Abbr‘s’,exten_insert_thm] >>
+‘?en ex. exten (IMAGE interval_bl P0) = (en,ex)’ by metis_tac[pairTheory.pair_CASES] >> simp[]>>
+‘?l0 d. interval_bl l = (l0,d)’ by metis_tac[pairTheory.pair_CASES] >> fs[] >>
+‘2 rpow -&LENGTH l = d’ by fsr[interval_bl_def] >> fs[] >>
+‘max (l0 + d) ex = d + max l0 (ex-d)’ by (fsr[max_def] >> rw[] >> fsr[]) >>fsr[GSYM REAL_ADD_ASSOC]>>
+‘?en'. (en,en') IN IMAGE interval_bl P0’ by metis_tac[exten_member,IMAGE_FINITE,IMAGE_EQ_EMPTY]>> fs[]>>
+rename[‘(en,en') = interval_bl EN’] >>
+‘l0+d<=en’ by (first_x_assum (qspecl_then [‘l’,‘EN’] mp_tac) >>
              simp[] >> impl_tac >- (strip_tac >> fs[GSYM DELETE_NON_ELEMENT])  >>
-             qpat_assum`interval_bl _ = _` (SUBST1_TAC o SYM) >> strip_tac >>
-             drule disjoint_interval_thm >> qpat_x_assum`_ = interval_bl _` (assume_tac o SYM)>>
+             qpat_assum‘interval_bl _ = _’ (SUBST1_TAC o SYM) >> strip_tac >>
+             drule disjoint_interval_thm >> qpat_x_assum‘_ = interval_bl _’ (assume_tac o SYM)>>
              simp[] >> strip_tac >>
-             `&TBL2N l * d <= bpos EN` by simp[] >> fs[interval_bl_def] >>rw[] >>
-             `0<2 rpow -&LENGTH EN` suffices_by fsr[] >> fs[RPOW_POS_LT]) >>
-`0 < d` by (rw[] >> fsr[RPOW_POS_LT]) >>
-`l0 <= en` by fsr[] >> simp[min_def] >>
-`en<=ex` by metis_tac[exten_low_high] >>
+             ‘&TBL2N l * d <= bpos EN’ by simp[] >> fs[interval_bl_def] >>rw[] >>
+             ‘0<2 rpow -&LENGTH EN’ suffices_by fsr[] >> fs[RPOW_POS_LT]) >>
+‘0 < d’ by (rw[] >> fsr[RPOW_POS_LT]) >>
+‘l0 <= en’ by fsr[] >> simp[min_def] >>
+‘en<=ex’ by metis_tac[exten_low_high] >>
 fsr[max_def] )
 
 val lemma1 = Q.prove(
-`(let is = IMAGE interval_bl P in !i1 i2. i1 IN is /\ i2 IN is /\ i1<>i2 ==> disjoint_interval i1 i2)
- ==>(!n. bls_size P n <= 1)`,
+‘(let is = IMAGE interval_bl P in !i1 i2. i1 IN is /\ i2 IN is /\ i1<>i2 ==> disjoint_interval i1 i2)
+ ==>(!n. bls_size P n <= 1)’,
 rw[EQ_IMP_THM,PULL_EXISTS] >> fs[bls_size_def,disjoint_interval_thm] >>
-`FINITE  {x | x IN P /\ LENGTH x < n}` by metis_tac[finite_and,finite_bool_list_lt_n] >>
-`FINITE {(\y. (&TBL2N y * 2 rpow -&LENGTH y,2 rpow -&LENGTH y)) x| x IN {z | z IN P /\ LENGTH z <n}}`
+‘FINITE  {x | x IN P /\ LENGTH x < n}’ by metis_tac[finite_and,finite_bool_list_lt_n] >>
+‘FINITE {(\y. (&TBL2N y * 2 rpow -&LENGTH y,2 rpow -&LENGTH y)) x| x IN {z | z IN P /\ LENGTH z <n}}’
  by metis_tac[IMAGE_FINITE,IMAGE_DEF] >> fs[] >>
-qabbrev_tac`s = {(&TBL2N x * 2 rpow -&LENGTH x,2 rpow -&LENGTH x) |  x IN P /\ LENGTH x < n}` >>
-Cases_on`s={}`
->- (`{x | x IN P /\ LENGTH x < n} = {}` by (fs[Abbr`s`] >>
-      `{(\y. (&TBL2N y * 2 rpow -&LENGTH y,2 rpow -&LENGTH y))  x | x IN P /\ LENGTH x < n} = {}`
+qabbrev_tac‘s = {(&TBL2N x * 2 rpow -&LENGTH x,2 rpow -&LENGTH x) |  x IN P /\ LENGTH x < n}’ >>
+Cases_on‘s={}’
+>- (‘{x | x IN P /\ LENGTH x < n} = {}’ by (fs[Abbr‘s’] >>
+      ‘{(\y. (&TBL2N y * 2 rpow -&LENGTH y,2 rpow -&LENGTH y))  x | x IN P /\ LENGTH x < n} = {}’
         by simp[] >>
-      `IMAGE (\x. (&TBL2N x * 2 rpow -&LENGTH x,2 rpow -&LENGTH x)) {x | x IN P /\ LENGTH x < n}
-        = {(\y. (&TBL2N y * 2 rpow -&LENGTH y,2 rpow -&LENGTH y))  x | x IN P /\ LENGTH x < n}`
+      ‘IMAGE (\x. (&TBL2N x * 2 rpow -&LENGTH x,2 rpow -&LENGTH x)) {x | x IN P /\ LENGTH x < n}
+        = {(\y. (&TBL2N y * 2 rpow -&LENGTH y,2 rpow -&LENGTH y))  x | x IN P /\ LENGTH x < n}’
         by fs[IMAGE_DEF] >> metis_tac[IMAGE_EQ_EMPTY]) >> fs[REAL_SUM_IMAGE_THM] ) >>
-`0<= FST (exten s) /\ SND (exten s) <= 1` by
-  (irule lemma11 >> rw[]>> fsr[Abbr`s`,TBL2N_lb,rpow_len_lb,TBL2N_ub2] >>
-   rw[] >> `x'<>x''` by (metis_tac[FUN_EQ_THM]) >>
-   `disjoint_interval (interval_bl x') (interval_bl x'')` by simp[] >>
-   `FST (interval_bl x') + SND (interval_bl x') <= FST (interval_bl x'') \/
-     FST (interval_bl x'') + SND (interval_bl x'') <= FST (interval_bl x')` by
+‘0<= FST (exten s) /\ SND (exten s) <= 1’ by
+  (irule lemma11 >> rw[]>> fsr[Abbr‘s’,TBL2N_lb,rpow_len_lb,TBL2N_ub2] >>
+   rw[] >> ‘x'<>x''’ by (metis_tac[FUN_EQ_THM]) >>
+   ‘disjoint_interval (interval_bl x') (interval_bl x'')’ by simp[] >>
+   ‘FST (interval_bl x') + SND (interval_bl x') <= FST (interval_bl x'') \/
+     FST (interval_bl x'') + SND (interval_bl x'') <= FST (interval_bl x')’ by
      simp[disjoint_interval_thm]  >> fs[interval_bl_def] ) >>
-qmatch_abbrev_tac`SIGMA f sn <= 1r`>> `SIGMA f sn <= SND (exten s)` suffices_by fsr[] >>
-`s = IMAGE interval_bl sn` by (fs[Abbr`sn`,Abbr`s`,interval_bl_def,IMAGE_DEF]) >> rw[] >>
-`!x x'. x IN sn /\ x' IN sn /\ x <> x' ==>
-             disjoint_interval (interval_bl x) (interval_bl x')` by
-  (`sn = P INTER {x | LENGTH x < n}` by fs[INTER_DEF] >> rw[]) >>
-Cases_on`sn={}` >> fs[REAL_SUM_IMAGE_THM] >>
-`SIGMA f sn + FST (exten (IMAGE interval_bl sn)) <= SND (exten (IMAGE interval_bl sn))` by
-  fs[Abbr`f`,lemma13] >> fsr[] )
+qmatch_abbrev_tac‘SIGMA f sn <= 1r’>> ‘SIGMA f sn <= SND (exten s)’ suffices_by fsr[] >>
+‘s = IMAGE interval_bl sn’ by (fs[Abbr‘sn’,Abbr‘s’,interval_bl_def,IMAGE_DEF]) >> rw[] >>
+‘!x x'. x IN sn /\ x' IN sn /\ x <> x' ==>
+             disjoint_interval (interval_bl x) (interval_bl x')’ by
+  (‘sn = P INTER {x | LENGTH x < n}’ by fs[INTER_DEF] >> rw[]) >>
+Cases_on‘sn={}’ >> fs[REAL_SUM_IMAGE_THM] >>
+‘SIGMA f sn + FST (exten (IMAGE interval_bl sn)) <= SND (exten (IMAGE interval_bl sn))’ by
+  fs[Abbr‘f’,lemma13] >> fsr[] )
 
 val kraft_ineq1 = Q.store_thm("kraft_ineq1",
-`!P. prefix_free P ==> (!n. bls_size P n <= 1)`,
+‘!P. prefix_free P ==> (!n. bls_size P n <= 1)’,
 (* Could change to `?y0. y0<=1 /\ bls_size P --> y0` *)
  metis_tac[disjoint_prefix_free,lemma1])
 
